dec_val HELL

refocusing_lang.v
@@ -5,13 +5,13 @@ Require Export Util.
 Module Type RED_LANG.
 
   (** The languages of terms, values, redex, and context, the empty context is also needed. *)
-  Parameters term ckind : Set. 
-  Parameters value redex elem_context : ckind -> Set.
-  Parameter  ckind_trans : forall k, elem_context k -> ckind.
+  Parameters term ckind elem_context : Set. 
+  Parameters value redex : ckind -> Set.
+  Parameter  ckind_trans : ckind -> elem_context -> ckind.
   Parameter  init_ckind : ckind.
   Inductive context : ckind -> ckind -> Set :=
-  | empty : forall k, context k k
-  | ccons : forall {k1} (ec : elem_context k1) {k2}, context k2 k1 -> context k2 (ckind_trans k1 ec).
+  | empty : forall {k}, context k k
+  | ccons : forall (ec : elem_context) {k1 k2}, context k1 k2 -> context k1 (ckind_trans k2 ec).
 
   (** The values and redexes are sublanguages of terms *)
   Parameter value_to_term : forall {k}, value k -> term.
@@ -26,25 +26,25 @@ Module Type RED_LANG.
   Fixpoint compose {k1 k2} (c0 : context k1 k2) {k3} (c1 : context k3 k1) : context k3 k2 := 
       match c0 in context k1' k2' return context k3 k1' -> context k3 k2' with
       | empty _ => fun c1' => c1'
-      | ccons _ ec _ c0' => fun c1' => ccons ec (compose c0' c1')
+      | ccons ec _ _ c0' => fun c1' => ccons ec (compose c0' c1')
       end c1.
-  Parameter atom_plug : term -> forall {k}, elem_context k -> term.
+  Parameter atom_plug : term -> elem_context -> term.
   Fixpoint plug (t : term) {k1 k2} (c : context k1 k2) : term := match c with
-  | empty _ => t | ccons _ ec _ c' => plug (atom_plug t ec) c' end.
+  | empty _ => t | ccons ec _ _ c' => plug (atom_plug t ec) c' end.
     
 
   (** The other main function of reduction semantics -- contraction of a redex into a term *)
   Parameter contract : forall {k}, redex k -> option term.
 
   Definition only_empty (t : term) (k : ckind) : Prop := 
-    forall t' k' (c : context k k'), plug t' c = t -> c ~= empty.
+    forall t' k' (c : context k k'), plug t' c = t -> k = k' /\ c ~= @empty k.
   Definition only_trivial (t : term) (k : ckind) : Prop := 
     forall t' k' (c : context k k'), plug t' c = t -> 
-      c ~= empty \/ exists (v : value k'), t' = value_to_term v.
+      k = k' /\ c ~= @empty k \/ exists (v : value k'), t' = value_to_term v.
 
   Axiom value_trivial : forall k (v : value k), only_trivial (value_to_term v) k.
   Axiom redex_trivial : forall k (r : redex k), only_trivial (redex_to_term r) k.
-  Axiom value_redex : forall k (v : value k) (r : redex k), value_to_term v <> redex_to_term r.
+  Axiom value_redex   : forall k (v : value k) (r : redex k), value_to_term v <> redex_to_term r.
   Axiom trivial_val_red : forall k (t : term), only_trivial t k ->
     (exists (v : value k), t = value_to_term v) \/ (exists (r : redex k), t = redex_to_term r).
 
@@ -58,7 +58,7 @@ Module Type RED_LANG.
   Inductive interm_dec k : Set :=
   | in_red  : redex k  -> interm_dec k
   | in_val  : value k -> interm_dec k
-  | in_term : term -> elem_context k -> interm_dec k.
+  | in_term : term -> elem_context -> interm_dec k.
 
   Arguments in_red {k} _. Arguments in_val {k} _. Arguments in_term {k} _ _.
 
@@ -72,10 +72,10 @@ End RED_LANG.
 
 Module Type LANG_PROP (R : RED_LANG).
 
-  Axiom plug_empty : forall t k, R.plug t (R.empty k) = t.
-  Axiom compose_empty : forall {k1 k2} (c : R.context k1 k2), c = R.compose c (R.empty _).
-  Axiom plug_compose : forall k1 k2 (c0 : R.context k1 k2) 
-                                 k3 (c1 : R.context k3 k1) (t : R.term), 
+  Axiom plug_empty : forall t k, R.plug t (@R.empty k) = t.
+  Axiom compose_empty : forall {k1 k2} (c : R.context k1 k2), c = R.compose c R.empty.
+  Axiom plug_compose : forall k1 k2 k3 (c0 : R.context k1 k2) (c1 : R.context k3 k1) 
+                               (t : R.term), 
                            R.plug t (R.compose c0 c1) = R.plug (R.plug t c0) c1.
 
 End LANG_PROP.
@@ -84,55 +84,54 @@ Module Type RED_REF_LANG.
 
   Declare Module R : RED_LANG.
 
-  Parameter dec_term    : R.term -> forall k, R.interm_dec k.
-  Parameter dec_context : forall {k} (ec : R.elem_context k), 
+  Parameter dec_term    : R.term -> forall k,  R.interm_dec k.
+  Parameter dec_context : forall (ec : R.elem_context) (k : R.ckind), 
                               R.value (R.ckind_trans k ec) -> R.interm_dec k.
 
   Inductive subterm_one_step : R.term -> R.term -> Prop :=
-  | st_1 : forall t t0 {k} (ec : R.elem_context k),
-               t = R.atom_plug t0 ec -> subterm_one_step t0 t.
+  | st_1 : forall t t0 ec, t = R.atom_plug t0 ec -> subterm_one_step t0 t.
   Axiom wf_st1 : well_founded subterm_one_step.
 
   Definition subterm_order := clos_trans_1n R.term subterm_one_step.
-  Notation " a <| b " := (subterm_order a b) (at level 40).
+  Notation " a <| b " := (subterm_order a b) (at level 40, no associativity).
   Definition wf_sto : well_founded subterm_order := wf_clos_trans_l _ _ wf_st1.
 
-  Parameter ec_order : forall {k}, R.elem_context k -> R.elem_context k -> Prop.
-  Notation " a <: b " := (ec_order a b) (at level 40).
-  Axiom wf_eco : forall {k}, well_founded (@ec_order k).
+  Parameter ec_order : R.ckind -> R.elem_context -> R.elem_context -> Prop.
+  Notation "k |-  a << b " := (ec_order k a b) (at level 40, no associativity).
+  Axiom wf_eco : forall k, well_founded (ec_order k).
 
   Axiom dec_term_red_empty  : forall t k (r : R.redex k), 
                                   dec_term t k = R.in_red r -> R.only_empty t k.
   Axiom dec_term_val_empty  : forall t k (v : R.value k), 
                                   dec_term t k = R.in_val v -> R.only_empty t k.
-  Axiom dec_term_term_top   : forall t t' k (ec : R.elem_context k), 
-            dec_term t k = R.in_term t' ec -> forall ec', ~ec <: ec'.
+  Axiom dec_term_term_top   : forall t t' k ec, 
+            dec_term t k = R.in_term t' ec -> forall ec', ~ k |- ec << ec'.
   Axiom dec_context_red_bot : forall k ec v r, 
-            @dec_context k ec v = @R.in_red k r -> forall ec', ~ ec' <: ec.
+            dec_context ec k v = R.in_red r -> forall ec', ~ k |- ec' << ec.
   Axiom dec_context_val_bot : forall k ec v v', 
-            @dec_context k ec v = @R.in_val k v' -> forall ec', ~ ec' <: ec.
+            dec_context ec k v = R.in_val v' -> forall ec', ~ k |- ec' << ec.
   Axiom dec_context_term_next : 
-    forall k ec v t ec', @dec_context k ec v = @R.in_term k t ec' -> 
-        ec' <: ec /\ forall ec'', ec'' <: ec -> ~ ec' <: ec''.
+    forall ec k v t ec', dec_context ec k v = R.in_term t ec' -> 
+        k |- ec' << ec /\ forall ec'', k |- ec'' << ec -> ~ k |- ec' << ec''.
 
-  Axiom dec_term_correct : forall k t, match dec_term t k with
+  Axiom dec_term_correct : forall t k, match dec_term t k with
     | R.in_red r => R.redex_to_term r = t
     | R.in_val v => R.value_to_term v = t
     | R.in_term t' ec => R.atom_plug t' ec = t
     end.
-  Axiom dec_context_correct : forall k ec v, match @dec_context k ec v with
+  Axiom dec_context_correct : forall ec k v, match dec_context ec k v with
     | R.in_red r => R.redex_to_term r = R.atom_plug (R.value_to_term v) ec
     | R.in_val v' => R.value_to_term v' = R.atom_plug (R.value_to_term v) ec
     | R.in_term t ec' => R.atom_plug t ec' = R.atom_plug (R.value_to_term v) ec
     end.
 
-  Axiom ec_order_antisym : forall k (ec ec0 : R.elem_context k), ec <: ec0 -> ~ ec0 <: ec.
-  Axiom dec_ec_ord : forall t0 t1 k ec0 ec1, 
-      @R.atom_plug t0 k ec0 = @R.atom_plug t1 k ec1 -> 
-      ec0 <: ec1 \/ ec1 <: ec0 \/ (t0 = t1 /\ ec0 = ec1).
+  Axiom ec_order_antisym : forall k (ec ec0 : R.elem_context), k |- ec << ec0 -> ~ k |- ec0 << ec.
+  (*Axiom dec_ec_ord : forall t0 t1 k ec0 ec1, 
+      R.atom_plug t0 ec0 = R.atom_plug t1 ec1 -> 
+      k |- ec0 << ec1 \/ k |- ec1 << ec0 \/ (t0 = t1 /\ ec0 = ec1).*)
   Axiom elem_context_det : forall t0 t1 k ec0 ec1, 
-    ec0 <: ec1 -> @R.atom_plug t0 k ec0 = @R.atom_plug t1 k ec1 ->
-    exists v, t1 = @R.value_to_term (R.ckind_trans k ec1) v.
+    k |- ec0 << ec1 -> R.atom_plug t0 ec0 = R.atom_plug t1 ec1 ->
+    exists v : R.value (R.ckind_trans k ec1), t1 = R.value_to_term v.
 
 End RED_REF_LANG.
 
