refocusing_signatures.v
@@ -5,24 +5,24 @@ Module Type RED_SEM (R : RED_LANG).
   Parameter dec : R.term -> forall {k1 k2}, R.context k1 k2 -> R.decomp k1 -> Prop.
 
   (** A redex in context will only ever be reduced to itself *)
-  Axiom dec_redex_self : forall k1 (r : R.redex k1) k2 (c : R.context k2 k1), 
+  Axiom dec_redex_self : forall k1 k2 (r : R.redex k2) (c : R.context k1 k2), 
                              dec (R.redex_to_term r) c (R.d_red r c).
 
-  Axiom decompose : forall (t : R.term) (k : R.ckind), 
-      (exists (v : R.value k), t = R.value_to_term v) \/
-      (exists k' (r : R.redex k') (c : R.context k k'), R.plug (R.redex_to_term r) c = t).
+  Axiom decompose : forall (t : R.term) (k1 : R.ckind), 
+      (exists (v : R.value k1), t = R.value_to_term v) \/
+      (exists k2 (r : R.redex k2) (c : R.context k1 k2), R.plug (R.redex_to_term r) c = t).
 
   (** dec is left inverse of plug *)
-  Axiom dec_correct : forall t {k1 k2} (c : R.context k1 k2) d, dec t c d -> 
+  Axiom dec_correct : forall k1 k2 t (c : R.context k1 k2) d, dec t c d -> 
       R.decomp_to_term d = R.plug t c.
 
   Axiom dec_plug : forall k1 k2 (c : R.context k1 k2) k3 (c0 : R.context k3 k1) t d, 
                        dec (R.plug t c) c0 d -> dec t (R.compose c c0) d.
-  Axiom dec_plug_rev : forall k1 k2 (c : R.context k1 k2) k3 (c0 : R.context k3 k1) t d, 
+  Axiom dec_plug_rev : forall k1 k2 k3 (c : R.context k1 k2) (c0 : R.context k3 k1) t d, 
                            dec t (R.compose c c0) d -> dec (R.plug t c) c0 d.
 
   Inductive decempty : R.term -> forall {k}, R.decomp k -> Prop :=
-  | d_intro : forall (t : R.term) k (d : R.decomp k), dec t (R.empty _) d -> decempty t d.
+  | d_intro : forall (t : R.term) {k} (d : R.decomp k), dec t (@R.empty k) d -> decempty t d.
 
   Inductive iter : forall {k}, R.decomp k -> R.value k -> Prop :=
   | i_val : forall {k} (v : R.value k), iter (R.d_val v) v
@@ -30,8 +30,8 @@ Module Type RED_SEM (R : RED_LANG).
               R.contract r = Some t -> decempty (R.plug t c) d -> iter d v ->
               iter (R.d_red r c) v.
 
-  Inductive eval : R.term -> forall k, R.value k -> Prop :=
-  | e_intro : forall t k d v, decempty t d -> iter d v -> eval t k v.
+  Inductive eval : R.term -> forall {k}, R.value k -> Prop :=
+  | e_intro : forall t {k} (d : R.decomp k) v, decempty t d -> iter d v -> eval t v.
 
 End RED_SEM.
 
@@ -39,49 +39,51 @@ Module Type RED_REF_SEM (R : RED_LANG).
 
   (** Functions specifying atomic steps of induction on terms and contexts -- needed to avoid explicit induction on terms and contexts in construction of the AM *)
   Parameter dec_term    : R.term -> forall k, R.interm_dec k.
-  Parameter dec_context : forall {k} (ec : R.elem_context k),
+  Parameter dec_context : forall (ec : R.elem_context) (k : R.ckind),
                               R.value (R.ckind_trans k ec) -> R.interm_dec k.
 
-  Axiom dec_term_correct : forall k t, match dec_term t k with
+  Axiom dec_term_correct : forall t k, match dec_term t k with
     | R.in_red r => R.redex_to_term r = t
     | R.in_val v => R.value_to_term v = t
     | R.in_term t0 ec0 => R.atom_plug t0 ec0 = t
   end.
-  Axiom dec_context_correct : forall k c v, match @dec_context k c v with
-    | R.in_red r => R.redex_to_term r = R.atom_plug (R.value_to_term v) c
-    | R.in_val v0 => R.value_to_term v0 = R.atom_plug (R.value_to_term v) c
-    | R.in_term t ec0 => R.atom_plug t ec0 = R.atom_plug (R.value_to_term v) c
+  Axiom dec_context_correct : forall ec k v, match dec_context ec k v with
+    | R.in_red r => R.redex_to_term r = R.atom_plug (R.value_to_term v) ec
+    | R.in_val v0 => R.value_to_term v0 = R.atom_plug (R.value_to_term v) ec
+    | R.in_term t ec0 => R.atom_plug t ec0 = R.atom_plug (R.value_to_term v) ec
   end.
 
   (** A decomposition function specified in terms of the atomic functions above *)
   Inductive dec : R.term -> forall {k1 k2}, R.context k1 k2 -> R.decomp k1 -> Prop :=
-  | d_dec  : forall (t : R.term) {k1 k2} (c : R.context k1 k2) (r : R.redex k2)
-               (DT  : dec_term t k2 = R.in_red r),
+  | d_dec  : forall t {k1 k2} (c : R.context k1 k2) (r : R.redex k2),
+               dec_term t k2 = R.in_red r -> 
                dec t c (R.d_red r c)
-  | d_v    : forall (t : R.term) {k1 k2} (c : R.context k1 k2) (v : R.value k2) (d : R.decomp k1)
-               (DT  : dec_term t k2 = R.in_val v)
-               (R_C : decctx v c d),
+  | d_v    : forall t {k1 k2} (c : R.context k1 k2) (v : R.value k2) (d : R.decomp k1),
+               dec_term t k2 = R.in_val v ->
+               decctx v c d ->
                dec t c d
-  | d_term : forall (t t0 : R.term) {k1 k2} (c : R.context k1 k2) (ec : R.elem_context k2) (d : R.decomp k1)
-               (DT  : dec_term t k2 = R.in_term t0 ec)
-               (R_T : dec t0 (R.ccons ec c) d),
+  | d_term : forall t t0 {k1 k2} (c : R.context k1 k2) ec (d : R.decomp k1),
+               dec_term t k2 = R.in_term t0 ec ->
+               dec t0 (R.ccons ec c) d ->
                dec t c d
   with decctx : forall {k2}, R.value k2 -> forall {k1}, R.context k1 k2 -> R.decomp k1 -> Prop :=
-  | dc_end  : forall {k} (v : R.value k), decctx v (R.empty _) (R.d_val v)
-  | dc_dec  : forall {k2} (ec : R.elem_context k2) v {k1} (c : R.context k1 k2) (r : R.redex k2),
-                dec_context ec v = R.in_red r ->
+  | dc_end  : forall {k} (v : R.value k), decctx v (@R.empty k) (R.d_val v)
+  | dc_dec  : forall ec {k2} (v : R.value (R.ckind_trans k2 ec)) 
+                        {k1} (c : R.context k1 k2) (r : R.redex k2),
+                dec_context ec k2 v = R.in_red r ->
                 decctx v (R.ccons ec c) (R.d_red r c)
-  | dc_val  : forall {k2} (v0 : R.value k2) (ec : R.elem_context k2) v {k1} (c : R.context k1 k2) 
-                         (d : R.decomp k1)
-                (DC  : dec_context ec v = R.in_val v0)
-                (R_C : decctx v0 c d),
+  | dc_val  : forall {k2} (v0 : R.value k2) ec   (v : R.value (R.ckind_trans k2 ec)) 
+                     {k1} (c  : R.context k1 k2) (d : R.decomp k1),
+                dec_context ec k2 v = R.in_val v0 ->
+                decctx v0 c d ->
                 decctx v (R.ccons ec c) d
-  | dc_term : forall {k2} (ec ec0 : R.elem_context k2) v {k1} (c : R.context k1 k2) (t : R.term) (d : R.decomp k1)
-                (DC  : dec_context ec v = R.in_term t ec0)
-                (R_T : dec t (R.ccons ec0 c) d),
+  | dc_term : forall ec ec0 {k2} (v : R.value (R.ckind_trans k2 ec)) 
+                            {k1} (c : R.context k1 k2) (t : R.term) (d : R.decomp k1),
+                dec_context ec k2 v = R.in_term t ec0 ->
+                dec t (R.ccons ec0 c) d ->
                 decctx v (R.ccons ec c) d.
 
-  Axiom dec_val_self : forall k2 (v : R.value k2) {k1} (c : R.context k1 k2) d, 
+  Axiom dec_val_self : forall k1 k2 (v : R.value k2) (c : R.context k1 k2) (d : R.decomp k1), 
       dec (R.value_to_term v) c d <-> decctx v c d.
 
   Declare Module RS : RED_SEM R with Definition dec := dec.
@@ -95,8 +97,10 @@ Module Type PE_REF_SEM (R : RED_LANG).
 
   Declare Module Red_Sem : RED_REF_SEM R.
 
-  Axiom dec_context_not_val : forall k v0 (ec : R.elem_context k) v, 
-            Red_Sem.dec_context ec v <> R.in_val v0. (* ??? *)
-  Axiom dec_term_value : forall k v, Red_Sem.dec_term (R.value_to_term v) k = R.in_val v.
+  (* Axiom dec_context_not_val : forall k (v0 : R.value k) (ec : R.elem_context) 
+                                       (v  : R.value (R.ckind_trans k ec)), 
+            Red_Sem.dec_context ec k v <> R.in_val v0. ??? *)
+  Axiom dec_term_value : forall k (v : R.value k), 
+                             Red_Sem.dec_term (R.value_to_term v) k = R.in_val v.
 
 End PE_REF_SEM.
