refocusing_substitutions.v
@@ -6,21 +6,23 @@ Require Import Program.
 
 Module Lang_Prop (R : RED_LANG) : LANG_PROP R.
 
-  Lemma plug_empty : forall t k, R.plug t (R.empty k) = t.
+  Lemma plug_empty : forall t k, R.plug t (@R.empty k) = t.
   Proof.
     intros; simpl; auto.
   Qed.
   Hint Resolve plug_empty : prop.
 
-  Lemma compose_empty : forall k1 k2 (c : R.context k1 k2), c = R.compose c (R.empty _).
+  Lemma compose_empty : forall k1 k2 (c : R.context k1 k2), c = R.compose c R.empty.
   Proof.
     intros. induction c. auto. simpl. rewrite<- IHc. auto.
   Qed.
   Hint Resolve compose_empty : prop.
 
-  Lemma plug_compose : forall k1 k2 (c : R.context k1 k2) k3 (c' : R.context k3 k1) (t : R.term), R.plug t (R.compose c c') = R.plug (R.plug t c) c'.
+  Lemma plug_compose : forall k1 k2 k3 (c : R.context k1 k2) (c' : R.context k3 k1) 
+                               (t : R.term), 
+                           R.plug t (R.compose c c') = R.plug (R.plug t c) c'.
   Proof.
-    intros ? ? ? ? ?. induction c; intro. auto. apply IHc.
+    intros ? ? ?. induction c; intros. auto. apply IHc.
   Qed.
   Hint Resolve plug_compose : prop.
 
@@ -29,83 +31,84 @@ End Lang_Prop.
 Module RedRefSem (R : RED_REF_LANG) <: RED_REF_SEM R.R.
 
   Definition dec_term := R.dec_term.
-  Definition dec_context := @R.dec_context. Arguments dec_context {k} _ _.
+  Definition dec_context := R.dec_context.
   Inductive dec : R.R.term -> forall {k1 k2}, R.R.context k1 k2 -> R.R.decomp k1 -> Prop :=
-  | d_dec  : forall (t : R.R.term) {k1 k2} (c : R.R.context k1 k2) (r : R.R.redex k2)
-               (DT  : dec_term t k2 = R.R.in_red r),
+  | d_dec  : forall t {k1 k2} (c : R.R.context k1 k2) (r : R.R.redex k2),
+               dec_term t k2 = R.R.in_red r -> 
                dec t c (R.R.d_red r c)
-  | d_v    : forall (t : R.R.term) {k1 k2} (c : R.R.context k1 k2) (v : R.R.value k2) (d : R.R.decomp k1)
-               (DT  : dec_term t k2 = R.R.in_val v)
-               (R_C : decctx v c d),
+  | d_v    : forall t {k1 k2} (c : R.R.context k1 k2) (v : R.R.value k2) (d : R.R.decomp k1),
+               dec_term t k2 = R.R.in_val v ->
+               decctx v c d ->
                dec t c d
-  | d_term : forall (t t0 : R.R.term) {k1 k2} (c : R.R.context k1 k2) (ec : R.R.elem_context k2) (d : R.R.decomp k1)
-               (DT  : dec_term t k2 = R.R.in_term t0 ec)
-               (R_T : dec t0 (R.R.ccons ec c) d),
+  | d_term : forall t t0 {k1 k2} (c : R.R.context k1 k2) ec (d : R.R.decomp k1),
+               dec_term t k2 = R.R.in_term t0 ec ->
+               dec t0 (R.R.ccons ec c) d ->
                dec t c d
   with decctx : forall {k2}, R.R.value k2 -> forall {k1}, R.R.context k1 k2 -> R.R.decomp k1 -> Prop :=
-  | dc_end  : forall {k} (v : R.R.value k), decctx v (R.R.empty _) (R.R.d_val v)
-  | dc_dec  : forall {k2} (ec : R.R.elem_context k2) v {k1} (c : R.R.context k1 k2) (r : R.R.redex k2),
-                dec_context ec v = R.R.in_red r ->
+  | dc_end  : forall {k} (v : R.R.value k), decctx v (@R.R.empty k) (R.R.d_val v)
+  | dc_dec  : forall ec {k2} (v : R.R.value (R.R.ckind_trans k2 ec)) 
+                        {k1} (c : R.R.context k1 k2) (r : R.R.redex k2),
+                dec_context ec k2 v = R.R.in_red r ->
                 decctx v (R.R.ccons ec c) (R.R.d_red r c)
-  | dc_val  : forall {k2} (v0 : R.R.value k2) (ec : R.R.elem_context k2) v {k1} (c : R.R.context k1 k2) 
-                         (d : R.R.decomp k1)
-                (DC  : dec_context ec v = R.R.in_val v0)
-                (R_C : decctx v0 c d),
+  | dc_val  : forall {k2} (v0 : R.R.value k2) ec   (v : R.R.value (R.R.ckind_trans k2 ec)) 
+                     {k1} (c  : R.R.context k1 k2) (d : R.R.decomp k1),
+                dec_context ec k2 v = R.R.in_val v0 ->
+                decctx v0 c d ->
                 decctx v (R.R.ccons ec c) d
-  | dc_term : forall {k2} (ec ec0 : R.R.elem_context k2) v {k1} (c : R.R.context k1 k2) (t : R.R.term) (d : R.R.decomp k1)
-                (DC  : dec_context ec v = R.R.in_term t ec0)
-                (R_T : dec t (R.R.ccons ec0 c) d),
+  | dc_term : forall ec ec0 {k2} (v : R.R.value (R.R.ckind_trans k2 ec)) 
+                            {k1} (c : R.R.context k1 k2) (t : R.R.term) (d : R.R.decomp k1),
+                dec_context ec k2 v = R.R.in_term t ec0 ->
+                dec t (R.R.ccons ec0 c) d ->
                 decctx v (R.R.ccons ec c) d.
 
   Scheme dec_Ind := Induction for dec Sort Prop
   with decctx_Ind := Induction for decctx Sort Prop.
     
   Notation " a <| b " := (R.subterm_order a b) (at level 40).
-  Notation " a <: b " := (R.ec_order a b) (at level 40).
+  Notation "k |-  a << b " := (R.ec_order k a b) (at level 40, no associativity).
 
   Lemma sto_trans : forall t t0 t1, t <| t0 -> t0 <| t1 -> t <| t1.
   Proof with auto.
     induction 1.
     econstructor 2; eauto.
-    econstructor 2; eauto; apply IHclos_trans_1n; auto.  
+    econstructor 2; eauto; apply IHclos_trans_1n; auto.
   Qed.
 
 
   Lemma plug_le_eq : forall k1 k2 (c : R.R.context k1 k2) t t0, R.R.plug t0 c = t -> 
-                         t0 <| t \/ (c ~= R.R.empty k1 /\ t = t0).
+                         t0 <| t \/ (c ~= @R.R.empty k1 /\ t = t0).
   Proof with auto.
     intros k1 k2.
     induction c; intros.
     simpl in H; right; auto.
-    left; simpl in H. destruct (IHc t (R.R.atom_plug t0 ec)); auto. Print t1n_trans.
+    left; simpl in H. destruct (IHc t (R.R.atom_plug t0 ec)); auto.
       apply t1n_trans with (y := R.R.atom_plug t0 ec). econstructor. reflexivity. assumption. 
       destruct H0. subst. rewrite H1. do 2 econstructor. reflexivity.
   Qed.
 
 
-  Lemma st_c : forall t0 t1, t0 <| t1 -> exists k1 k2 (c : R.R.context k1 k2), R.R.plug t0 c = t1.
-  (* zonk *)
-
+  Lemma st_c : forall t0 t1, t0 <| t1 -> 
+                   forall k1, exists k2 (c : R.R.context k1 k2), R.R.plug t0 c = t1.
   Proof with auto.
-    intros t0 t1 H. induction H. inversion H; subst.
-    exists (R.R.ccons ec R.R.empty); simpl; auto.
-    destruct IHclos_trans_n1 as [c H1].
-    exists (c ++ (existT _ k ec :: nil)); unfold R.R.plug in *; rewrite fold_left_app; simpl; subst; auto.
+    intros t0 t1 H k1. induction H; intros. inversion H; subst. 
+    exists (R.R.ckind_trans k1 ec). exists (R.R.ccons ec (@R.R.empty k1)); simpl; auto.
+    destruct IHclos_trans_1n as [k2 [c H1]]. inversion H; subst.
+    exists (R.R.ckind_trans k2 ec). exists (R.R.ccons ec c). auto.
   Qed.
-
-  Definition value_one_step {k} (v v0 : R.R.value k) : Prop := 
+(*
+  Definition value_one_step {k1} (v : R.R.value k1) {k2} (v0 : R.R.value k2) : Prop := 
       R.subterm_one_step (R.R.value_to_term v) (R.R.value_to_term v0).
-  Definition value_order k := clos_trans_n1 (R.R.value k) value_one_step.
+  Definition value_order k := clos_trans_1n (R.R.value k) value_one_step.
     
-  Notation " a <v| b " := (value_order a b) (at level 40).
+  Notation "k |- a <v| b" := (@value_order k a b) (at level 40).
     
   Lemma wf_vo : forall {k}, well_founded (value_order k).
   Proof.
     intro k.
-    apply wf_clos_trans_r. unfold value_one_step. apply wf_inverse_image. apply R.wf_st1.
+    apply wf_clos_trans_l. unfold value_one_step. apply wf_inverse_image. apply R.wf_st1.
   Qed.
-
-    Reserved Notation " a <v| b " (at level 40).
+*)
+    (*Reserved Notation " a <v| b " (at level 40).
 
     Inductive value_order : R.R.value -> R.R.value -> Prop :=
     | vc_1 : forall v0 v1 ec (ATOM: R.R.atom_plug (R.R.value_to_term v0) ec = (R.R.value_to_term v1)), v0 <v| v1
@@ -119,23 +122,134 @@ Module RedRefSem (R : RED_REF_LANG) <: RED_REF_SEM R.R.
       apply wf_incl with hp.
       unfold inclusion; intros; induction H; [ econstructor | econstructor 2]; eauto; econstructor; eauto.
       apply wf_inverse_image; apply R.wf_sto.
-    Qed.
+    Qed.*)
 
-    Lemma dec_val : forall {k} (v : R.R.value k) (c : R.R.context k) (d : R.R.decomp), dec (R.R.value_to_term v) c d -> decctx v c d.
+
+
+
+(* REFACTOR *)
+
+Require Import Coq.Logic.EqdepFacts.
+
+Definition JMeq_eq_depT := 
+fun (U : Type) (P : U -> Type) (p q : U) (x : P p) (y : P q) (H : p = q)
+  (H0 : x ~= y) =>
+match
+  H in (_ = y0) return (forall y1 : P y0, x ~= y1 -> eq_dep U P p x y0 y1)
+with
+| eq_refl =>
+    fun (y0 : P p) (H1 : x ~= y0) =>
+    (fun H2 : x = y0 =>
+     eq_ind_r (fun x0 : P p => eq_dep U P p x0 p y0) (eq_dep_intro U P p y0)
+       H2) (JMeq_eq H1)
+end y H0.
+
+Lemma ccons_inj : forall ec {k1 k2} c ec' {k2'} c', 
+R.R.ckind_trans k2 ec = R.R.ckind_trans k2' ec' ->
+@R.R.ccons ec k1 k2 c ~= @R.R.ccons ec' k1 k2' c' ->
+ec = ec' /\ k2 = k2' /\ c ~= c'.
+Proof.
+intros.
+assert (H1 := JMeq_eq_depT _ _ _ _ _ _ H H0).
+assert (H2 := eq_dep_eq_sigT _ _ _ _ _ _ H1). 
+inversion H2; subst.
+assert (H7' := inj_pair2 _ _ _ _ _ H7); subst; clear H7.
+assert (H7'' := inj_pair2 _ _ _ _ _ H7'); subst; clear H7'.
+auto.
+Qed.
+
+(*
+Lemma decctx_des : forall ec {k2} (v : R.R.value (R.R.ckind_trans k2 ec)) 
+                             {k1} (c : R.R.context k1 k2) (d : R.R.decomp k1),
+                             decctx v (R.R.ccons ec c) d ->
+
+  (exists r, d = R.R.d_red r c /\ R.dec_context ec k2 v = R.R.in_red r) \/
+  (exists v0, R.dec_context ec k2 v = R.R.in_val v0 /\ decctx v0 c d) \/
+  (exists ec0 t, R.dec_context ec k2 v = R.R.in_term t ec0 /\
+                 dec t (R.R.ccons ec0 c) d).
+Proof.
+intros.
+dependent destruction H;
+assert (H1 := xxx _ _ _ _ _ _ _ x0 x);
+
+destruct H1 as (H1a,(H1b, H1c)); destruct H1a; destruct H1b; subst.
+
+left; exists r; auto.
+
+right; left; exists v0; auto.
+
+right; right; exists ec1; exists t; auto.
+Qed.
+*)
+    Lemma dec_val : forall k1 k2 (v : R.R.value k2) (c : R.R.context k1 k2) (d : R.R.decomp k1), 
+                        dec (R.R.value_to_term v) c d -> decctx v c d.
     Proof with eauto.
-      intro k.
-      induction v using (well_founded_ind wf_vo); intros.
+      intros k1 k2 v.
+      remember (R.R.value_to_term v). revert k2 v Heqt.
+      induction t using (well_founded_ind R.wf_sto); intros.
+      rewrite Heqt in H0.
 
       dependent destruction H0; unfold dec_term in *;
-      assert (hh := R.dec_term_correct k (R.R.value_to_term v)); rewrite DT in hh.
+      assert (hh := R.dec_term_correct (R.R.value_to_term v) k2); rewrite H0 in hh.
 
       symmetry in hh; contradiction (R.R.value_redex _ _ _ hh).
 
       rewrite<- (R.R.value_to_term_injective _ _ _ hh).
       assumption.
 
-      destruct (R.R.value_trivial v t (e :: nil)); simpl...
-      discriminate H1.
+      destruct (R.R.value_trivial _ v t1 _ (R.R.ccons ec R.R.empty)); simpl; auto;
+      destruct H2.
+
+      assert (eq_dep _ _ (R.R.ckind_trans k2 ec) (R.R.ccons ec (@R.R.empty k2)) k2 (@R.R.empty k2)).
+
+
+      apply JMeq_eq_depT; auto.
+      discriminate (eq_dep_eq_sigT _ _ _ _ _ _ H4).
+      
+      assert (decctx x (R.R.ccons ec c) d).
+
+      apply (H t1).
+      do 2 econstructor 1.
+      rewrite<- hh in Heqt.
+      apply Heqt.
+      auto.
+      auto.
+
+      dependent destruction H3;
+      assert (G1 := ccons_inj _ _ _ _ x1 x);
+      destruct G1 as (G1a,(G1b, G1c)); destruct G1a; destruct G1b; subst;
+      unfold dec_context in *;
+
+      assert (gg := R.dec_context_correct ec0 k0 x0); rewrite H3 in gg.
+
+      contradiction (R.R.value_redex _ v r).
+      transitivity (R.R.atom_plug (R.R.value_to_term x0) ec0); auto.
+
+      assert (v0 = v).
+      apply (R.R.value_to_term_injective _ v0 v ).
+      transitivity (R.R.atom_plug (R.R.value_to_term x0) ec0); auto.
+      subst; auto.
+
+clear x H x1 H4 H1 gg.
+      revert v H0 hh.
+      induction ec0 using (well_founded_ind (R.wf_eco k0)); intros.
+      assert (HH := H 
+
+      inversion H3.
+      subst.
+      assert (H13' := inj_pair2 _ _ _ _ _ H13); subst; clear H13.
+      assert (H7' := inj_pair2 _ _ _ _ _ H7); subst; clear H7.
+      assert (H12' := inj_pair2 _ _ _ _ _ H12); 
+      assert (H12'' := inj_pair2 _ _ _ _ _ H12'); subst; clear H4 H5 H9 H12 H12'.
+      assert (gg := R.dec_context_correct ec k2 v1). unfold dec_context in *.
+      rewrite H8 in gg.
+      rewrite x2 in *.
+      constructor 2.
+      
+      rewrite<- H3.
+      generalize k2 at 5.
+      rewrite<- H2.
+      discriminate H2.
       destruct H1 as [v0 H1]; subst t.
       symmetry in hh; assert (ht := R.st_1 _ _ _ hh);
       apply (tn1_step _ value_one_step) in ht; change (v0 <v| v) in ht.
